src/coq/DynamicTypes.v
@@ -67,14 +67,14 @@ Section hiding_notation.
     | DTYPE_Metadata  => Raw "metadata"
     | DTYPE_X86_mmx   => Raw "x86_mmx"
     | DTYPE_Array sz t
-      => [Raw "[" ; to_sexp sz ; Raw "x" ; serialize_dtyp' t ; Raw "]"]
+      => [Raw ("[" ++ to_string sz) ; Raw "x" ; serialize_dtyp' t ; Raw "]"]
     | DTYPE_Struct fields
       => [Raw "{" ; to_sexp (List.map (fun x => [serialize_dtyp' x ; Raw ","]) fields) ; Raw "}"]
     | DTYPE_Packed_struct fields
       => [Raw "packed{" ; to_sexp (List.map (fun x => [serialize_dtyp' x ; Raw ","]) fields) ; Raw "}"]
     | DTYPE_Opaque => Raw "opaque"
     | DTYPE_Vector sz t
-      => [Raw "<" ; to_sexp sz ; Raw "x" ; serialize_dtyp' t ; Raw ">"]  (* TODO: right notation? *)
+      => [Raw ("<" ++ to_string sz) ; Raw "x" ; serialize_dtyp' t ; Raw ">"]  (* TODO: right notation? *)
     end.
 
   Global Instance serialize_dtyp : Serialize dtyp := serialize_dtyp'.
